Memory.v
@@ -1,0 +1,59 @@
+(* Janus Memories formalized *)
+
+Require Import Arith.
+Require Import Word32.
+
+Section Memory.
+  (* Variables are natural numbers *)
+  Definition var := nat.
+  (* Memories are maps from variables to w32 optional types *)
+  Definition memory := var -> option w32.
+  (* The default store fails any lookup *)
+  Definition empty (_ : var) : option w32 := None.
+
+  (* Write [v] to memory location [x] in memory [m] *)
+  Definition write (m : memory) x v x' :=
+    if eq_nat_dec x x'
+      then Some v
+      else m x'.
+
+  Definition hide (m : memory) x x' :=
+    if eq_nat_dec x x'
+      then None
+      else m x'.
+
+  (* Proof automation hints *)
+  Lemma write_eq : forall m a v, write m a v a = Some v.
+    unfold write.
+    intros.
+    destruct (eq_nat_dec a a); tauto.
+  Qed.
+
+  Hint Rewrite write_eq : write.
+
+  Lemma write_ne : forall m a v a', a <> a'
+    -> write m a v a' = m a'.
+    unfold write.
+    intros.
+    destruct (eq_nat_dec a a'); tauto.
+  Qed.
+
+  Hint Rewrite write_ne using omega : write.
+
+  Lemma write_eq_2 : forall m m' a v v',
+    write m a v a = write m' a v' a -> v = v'.
+  Proof.
+    unfold write. intros. destruct (eq_nat_dec a a). injection H. trivial.
+    contradiction n. trivial.
+  Qed.
+
+  Lemma write_eq_3 : forall m m' a v v' x,
+    write m a v x = write m' a v' x -> v = v' \/ m x = m' x.
+    unfold write. intros. destruct (eq_nat_dec a x). injection H. auto.
+    auto.
+  Qed.
+
+  (* Want to prove a number of propositions on stores/memories here
+     to make it possible to do full backwards determinism. *)
+
+End Memory.
